Make good progress in the proof of [blake2_is_hash_incremental]

specs/lemmas/Spec.Hash.Incremental.fst
@@ -22,7 +22,7 @@ let add_v_eq (a b : nat) :
   (requires (a + b <= pow2 64 - 1))
   (ensures (v (u64 a +. u64 b) == a + b)) = ()
 
-/// The [blake2_is_hash_incremental] lemma is not fundamentally difficult, but
+/// The [repeati_blake2_update1_as_update_multi_eq] lemma is not fundamentally difficult, but
 /// the proof time/success rate can be very random, probably because of modular
 /// arithmetic. For this reason, we cut it into small pieces.
 let update_multi_one_block_eq
@@ -68,7 +68,7 @@ let repeati_blake2_update1_eq
     nb > 0 /\
     nb * block_length a <= Seq.length d /\
     prev + nb * block_length a <= max_limb (to_blake_alg a) /\
-    nb < Seq.length d / size_block (to_blake_alg a) /\
+    nb <= Seq.length d / size_block (to_blake_alg a) /\
     prev + Seq.length d <= max_limb (to_blake_alg a) /\
     prev + nb * block_length a <= pow2 64 - 1
   ))
@@ -83,7 +83,7 @@ let repeati_blake2_update1_eq
   let block = S.slice d ((nb-1) * block_length a) (nb * block_length a) in
   Loops.unfold_repeati nb update1 hash (nb - 1)
 
-/// TODO: the time spent on this proof is very random.
+/// TODO: the time spent on this proof is super random.
 #push-options "--z3rlimit 500 --fuel 1"
 let rec repeati_blake2_update1_as_update_multi_eq
   (a:hash_alg{is_blake a}) (nb prev : nat)
@@ -93,7 +93,7 @@ let rec repeati_blake2_update1_as_update_multi_eq
   (requires (
     nb * block_length a <= Seq.length d /\
     prev + nb * block_length a <= max_limb (to_blake_alg a) /\
-    nb < Seq.length d / size_block (to_blake_alg a) /\
+    nb <= Seq.length d / size_block (to_blake_alg a) /\
     prev + Seq.length d <= max_limb (to_blake_alg a) /\
     prev + nb * block_length a <= pow2 64 - 1
   ))
@@ -131,12 +131,385 @@ let rec repeati_blake2_update1_as_update_multi_eq
     end
 #pop-options
 
+/// Once again, proof times are random...
+(* let blake2_no_finish_no_last
+  (a:hash_alg{is_blake a}) (input:bytes{Seq.length input <= max_input_length a}) =
+  let nn = Spec.Blake2.max_output (to_blake_alg a) in
+  let prev0 = compute_prev0 (to_blake_alg a) 0 in
+  let s1 = blake2_init (to_blake_alg a) 0 Seq.empty nn in
+  let (nb,rem) = split (to_blake_alg a) (S.length input) in
+  let s2 = Loops.repeati nb (blake2_update1 (to_blake_alg a) prev0 input) s1 in
+  s2
+
+let blake2_ihash_no_finish_no_last
+  (a:hash_alg{is_blake a}) (input:bytes{Seq.length input <= max_input_length a}) =
+  let bs, l = split_blocks a input in
+  let is1 = init a in
+  let is2 = update_multi a is1 bs in
+  is2 *)
+
+let blake2_no_finish
+  (a:hash_alg{is_blake a}) (input:bytes{Seq.length input <= max_input_length a}) =
+  let nn = Spec.Blake2.max_output (to_blake_alg a) in
+  let prev0 = compute_prev0 (to_blake_alg a) 0 in
+  let s1 = blake2_init (to_blake_alg a) 0 Seq.empty nn in
+  let (nb,rem) = split (to_blake_alg a) (S.length input) in
+  let s2 = Loops.repeati nb (blake2_update1 (to_blake_alg a) prev0 input) s1 in
+  let s3 = blake2_update_last (to_blake_alg a) prev0 rem input s2 in
+  s3
+
+let blake2_ihash_no_finish
+  (a:hash_alg{is_blake a}) (input:bytes{Seq.length input <= max_input_length a}) =
+  let bs, l = split_blocks a input in
+  let is1 = init a in
+  let is2 = update_multi a is1 bs in
+  let is3 = update_last a is2 (S.length bs) l in
+  is3
+
+
+(* TODO HERE *)
+/// Sanity check
+#push-options "--z3rlimit 500 --fuel 0 --ifuel 0"
+let blake2_is_hash_incremental_aux
+  (a:hash_alg{is_blake a}) (input:bytes{Seq.length input <= max_input_length a})
+  : Lemma
+    (blake2_no_finish a input == fst (blake2_ihash_no_finish a input))
+  =
+  (* Let's prove the equality step by step *)
+  (**)
+  let nn = Spec.Blake2.max_output (to_blake_alg a) in
+  let prev0 = compute_prev0 (to_blake_alg a) 0 in
+  let s1 = blake2_init (to_blake_alg a) 0 Seq.empty nn in
+  let (nb,rem) = split (to_blake_alg a) (S.length input) in
+  let s2 = Loops.repeati nb (blake2_update1 (to_blake_alg a) prev0 input) s1 in
+  let s3 = blake2_update_last (to_blake_alg a) prev0 rem input s2 in
+  (**)
+  let bs, l = split_blocks a input in
+  let is1 = init a in
+  let is2 = update_multi a is1 bs in
+  let is3 = update_last a is2 (S.length bs) l in
+  (* [s1 == fst is1] *)
+  assert(s1 == fst is1);
+  (* [s2 == fst is2] *)
+  assert(S.length bs == nb * block_length a);
+  assert(
+    nb * block_length a <= Seq.length input /\
+    prev0 + nb * block_length a <= max_limb (to_blake_alg a) /\
+    nb <= Seq.length input / size_block (to_blake_alg a) /\
+    prev0 + Seq.length input <= max_limb (to_blake_alg a) /\
+    prev0 + nb * block_length a <= pow2 64 - 1);
+  repeati_blake2_update1_as_update_multi_eq a nb prev0 input s1;  
+  assert(s2 == fst is2);
+  (* [s3 == fst is3] *)
+  (* First, work on [s3] *)
+  assert(rem == S.length input - S.length bs);
+  assert(l `S.equal` S.slice input (S.length input - rem) (S.length input));
+  let pblock1 = get_last_padded_block (to_blake_alg a) input rem in
+//  assert(
+//    forall (i:nat{i < S.length l}). S.index pblock1 i == S.index l i);
+//  assert(
+//    forall (i:nat{S.length l <= i /\ i < block_length a}).
+//      S.index pblock1 i == S.index (S.create (block_length a) (u8 0)) i);
+  assume(
+    get_last_padded_block (to_blake_alg a) input rem `S.equal`
+      Seq.append l (S.create (block_length a - S.length l) (u8 0)));
+  assert(
+    s3 == blake2_update_block (to_blake_alg a) true (S.length input) pblock1 s2);
+  (* Then, work on [is3] *)
+  assert(
+    is3 == update_last_blake a is2 (S.length bs) l);
+  let blocks, last_block, rem' = last_split_blake a l in
+  assert(
+    blocks == S.empty /\
+    last_block == Spec.Blake2.get_last_padded_block (to_blake_alg a) l rem /\
+    rem' = S.length l);
+//  assert(
+//    last_split_blake a l ==
+//    (S.empty, Spec.Blake2.get_last_padded_block (to_blake_alg a) l rem, S.length l));
+  let h' = update_multi a is2 S.empty in
+  update_multi_zero a is2;
+  assert(h' == is2);
+  assert(snd h' == u64 (S.length bs));
+  assume(v (snd h' +. u64 rem) == S.length input);
+  assert(
+    is3 ==
+    (Spec.Blake2.blake2_update_block (to_blake_alg a) true (v (snd h' +. u64 rem))
+                                     last_block (fst h'),
+     u64 0));
+  (* Prove the final equality *)
+  assert(s3 == fst is3)
+
 (*
-#push-options "--z3rlimit 500 --ifuel 1"
+let split (a:alg) (len:nat)
+  : nb_rem:(nat & nat){let (nb,rem) = nb_rem in
+		   nb * size_block a + rem == len} =
+  let nb = len / size_block a in
+  let rem = len % size_block a in
+  let nb' = if rem = 0 && nb > 0 then nb - 1 else nb in
+  let rem' = if rem = 0 && nb > 0 then size_block a else rem in
+  (nb',rem')
+
+let last_split_blake (a:hash_alg{is_blake a}) (input:bytes)
+  : Pure (bytes & bytes & nat)
+    (requires True)
+    (ensures fun (b, l, rem) ->
+      S.length b % block_length a == 0 /\
+      S.length l == block_length a /\
+      rem <= block_length a /\
+      rem <= S.length input)
+  = let (nb, rem) = Spec.Blake2.split (to_blake_alg a) (S.length input) in
+    let blocks = Seq.slice input 0 (nb * block_length a) in
+    let last_block = Spec.Blake2.get_last_padded_block (to_blake_alg a) input rem in
+    blocks, last_block, rem
+
+let update_last_blake (a:hash_alg{is_blake a})
+  (hash:words_state a)
+  (prevlen:nat{prevlen % block_length a = 0})
+  (input:bytes{S.length input + prevlen <= max_input_length a}):
+  Tot (words_state a)
+  = let blocks, last_block, rem = last_split_blake a input in
+    let h' = update_multi a hash blocks in
+    (Spec.Blake2.blake2_update_block (to_blake_alg a) true (v (snd h' +. u64 rem)) last_block (fst h'), u64 0)
+
+
+  assert(
+    is3 == update_last_blake a is2 (S.length bs) l);
+  assert(
+    last_split_blake a l ==
+      bs, 
+  admit()
+
+  assert(
+    let last_pblock = Spec.Blake2.get_last_padded_block (to_blake_alg a) input rem in
+    last_split_blake a is2 (S.length bs) l == bs, last_pblock, rem
+
+let blake2_update_last a prev rem m s =
+  let inlen = length m in
+  let totlen = prev + inlen in
+  let last_block = get_last_padded_block a m rem in
+  blake2_update_block a true totlen last_block s (**)
+
+let get_last_padded_block (a:alg) (m:bytes)
+    (rem:nat{rem <= length m /\ rem <= size_block a}) : block_s a =
+  let last = Seq.slice m (length m - rem) (length m) in
+  let last_block = create (size_block a) (u8 0) in
+  let last_block = update_sub last_block 0 rem last in
+  last_block
+
+(**)
+
+let update_last (a:hash_alg)
+  (hash:words_state a)
+  (prevlen:nat{prevlen % block_length a = 0})
+  (input:bytes{S.length input + prevlen <= max_input_length a}):
+  Tot (words_state a)
+=
+    update_last_blake a hash prevlen input
+
+
+let last_pblock = Spec.Blake2.get_last_padded_block (to_blake_alg a) input rem in
+update_last_blake == bs, last_pblock, rem
+                     
+
+  assert(s3 == is3)
+#pop-options
+
+
+/// Sanity check
+#push-options "--z3rlimit 50 --fuel 0 --ifuel 0"
+let blake2_init_eq
+  (a:hash_alg{is_blake a}) (input:bytes{Seq.length input <= max_input_length a})
+  : Lemma (
+      (**)
+      let nn = Spec.Blake2.max_output (to_blake_alg a) in
+      let prev0 = compute_prev0 (to_blake_alg a) 0 in
+      let s1 = blake2_init (to_blake_alg a) 0 Seq.empty nn in
+      (**)
+      let bs, l = split_blocks a input in
+      let is1 = init a in
+      (**)
+      s1 == fst is1)
+  = ()
+#pop-options
+
+/// Sanity check
+#push-options "--z3rlimit 500 --fuel 0 --ifuel 0"
+let blake2_is_hash_incremental_aux
+  (a:hash_alg{is_blake a}) (input:bytes{Seq.length input <= max_input_length a})
+  : Lemma
+    (requires (blake2_no_finish a input == fst (blake2_ihash_no_finish a input)))
+    (ensures (
+      Spec.Blake2.blake2 (to_blake_alg a) input 0 Seq.empty
+                        (Spec.Blake2.max_output (to_blake_alg a)) ==
+      hash_incremental a input))
+  = ()
+#pop-options
+
+/// It is enough to prove the requirement of the above lemma
+let blake2_no_finish_eq
+  (a:hash_alg{is_blake a}) (input:bytes{Seq.length input <= max_input_length a}) :
+  Lemma(blake2_no_finish a input == fst (blake2_ihash_no_finish a input)) =
+  (**)
+  let nn = Spec.Blake2.max_output (to_blake_alg a) in
+  let prev0 = compute_prev0 (to_blake_alg a) 0 in
+  let s1 = blake2_init (to_blake_alg a) 0 Seq.empty nn in
+  let (nb,rem) = split (to_blake_alg a) (S.length input) in
+  let s2 = Loops.repeati nb (blake2_update1 (to_blake_alg a) prev0 input) s1 in
+  (**)
+  let bs, l = split_blocks a input in
+  let is1 = init a in
+  let is2 = update_multi a is1 bs in
+  let is3 = update_last a is2 (S.length bs) l in
+  (**)
+  
+  
+
+let blake2_no_finish
+  (a:hash_alg{is_blake a}) (input:bytes{Seq.length input <= max_input_length a}) =
+  let nn = Spec.Blake2.max_output (to_blake_alg a) in
+  let prev0 = compute_prev0 (to_blake_alg a) 0 in
+  let s1 = blake2_init (to_blake_alg a) 0 Seq.empty nn in
+  let (nb,rem) = split (to_blake_alg a) (S.length input) in
+  let s2 = Loops.repeati nb (blake2_update1 (to_blake_alg a) prev0 input) s1 in
+  let s3 = blake2_update_last (to_blake_alg a) prev0 rem input s2 in
+  s3
+
+let blake2_ihash_no_finish
+  (a:hash_alg{is_blake a}) (input:bytes{Seq.length input <= max_input_length a}) =
+  let bs, l = split_blocks a input in
+  let is1 = init a in
+  let is2 = update_multi a is1 bs in
+  let is3 = update_last a is2 (S.length bs) l in
+  is3
+
+
+#push-options "--z3rlimit 500 --fuel 0 --ifuel 0"
 let blake2_is_hash_incremental
   (a:hash_alg{is_blake a}) (input:bytes{Seq.length input <= max_input_length a})
   : Lemma
-    (Spec.Blake2.blake2 (to_blake_alg a) input 0 Seq.empty (Spec.Blake2.max_output (to_blake_alg a)) ==
+    (Spec.Blake2.blake2 (to_blake_alg a) input 0 Seq.empty
+                        (Spec.Blake2.max_output (to_blake_alg a)) ==
+     hash_incremental a input)
+  =
+  (* Different steps for original blake spec *)
+  let nn = Spec.Blake2.max_output (to_blake_alg a) in
+  let prev0 = compute_prev0 (to_blake_alg a) 0 in
+  let s1 = blake2_init (to_blake_alg a) 0 Seq.empty nn in
+//  let s2 = blake2_update_blocks (to_blake_alg a) prev0 input s1 in
+  let (nb,rem) = split (to_blake_alg a) (S.length input) in
+  let s2 = Loops.repeati nb (blake2_update1 (to_blake_alg a) prev0 input) s1 in
+  let s3 = blake2_update_last (to_blake_alg a) prev0 rem input s2 in
+  let s3' = blake2_update_blocks (to_blake_alg a) prev0 input s1 in
+  assume(s3' == s3);
+  let s4 = blake2_finish (to_blake_alg a) s3 nn in
+  let s4' = Spec.Blake2.blake2 (to_blake_alg a) input 0 Seq.empty
+                               (Spec.Blake2.max_output (to_blake_alg a)) in
+  assume(s4 == s4');
+  (* Different steps for blake incremental *)
+  let bs, l = split_blocks a input in
+  let is1 = init a in
+  assume(S.length bs % block_length a == 0);
+  let is2 = update_multi a is1 bs in
+//  assume(S.length bs % block_length a == 0);
+  let is3 = update_last a is2 (S.length bs) l in (**)
+  let is4 = finish a is3 in
+  let is4' = hash_incremental a input in
+  assume(is4' == is4);
+  (* Let's show that is2 == s3 (suffices to prove the goal) *)
+  assume(fst is3 == s3)
+#pop-options
+
+#push-options "--z3rlimit 1000"
+let blake2_is_hash_incremental
+  (a:hash_alg{is_blake a}) (input:bytes{Seq.length input <= max_input_length a})
+  : Lemma
+    (Spec.Blake2.blake2 (to_blake_alg a) input 0 Seq.empty
+                        (Spec.Blake2.max_output (to_blake_alg a)) ==
+     hash_incremental a input)
+  =
+  (* Different steps for original blake spec *)
+  let nn = Spec.Blake2.max_output (to_blake_alg a) in
+  let prev0 = compute_prev0 (to_blake_alg a) 0 in
+  let s1 = blake2_init (to_blake_alg a) 0 Seq.empty nn in
+  let s2 = blake2_update_blocks (to_blake_alg a) prev0 input s1 in
+//  let (nb,rem) = split (to_blake_alg a) (S.length input) in
+//  let s2 = Loops.repeati nb (blake2_update1 (to_blake_alg a) prev0 input) s1 in
+//  let s3 = blake2_update_last (to_blake_alg a) prev0 rem input s2 in
+//  let s3' = blake2_update_blocks (to_blake_alg a) prev0 input s1 in
+//  assert(s3' == s3);
+  let s4 = blake2_finish (to_blake_alg a) s2 nn in
+  let s4' = Spec.Blake2.blake2 (to_blake_alg a) input 0 Seq.empty
+                               (Spec.Blake2.max_output (to_blake_alg a)) in
+  assert(s4 == s4');
+  (* Different steps for blake incremental *)
+  let bs, l = split_blocks a input in
+  let is1 = update_multi a (init a) bs in
+  let is2 = update_last a is1 (S.length bs) l in
+  let is3 = finish a is2 in
+  let is3' = hash_incremental a input in
+  assert(is3' == is3);
+  (* Let's show that is2 == s3 (suffices to prove the goal) *)
+  assume(fst is2 == s2)
+#pop-options
+
+
+let hash_incremental (a:hash_alg) (input:bytes{S.length input <= (max_input_length a)}):
+  Tot (hash:bytes{S.length hash = (hash_length a)})
+=
+  let bs, l = split_blocks a input in
+  let hash = update_multi a (init a) bs in
+  let hash = update_last a hash (S.length bs) l in
+  finish a hash
+  
+
+
+  let open FStar.Mul in
+  let n = S.length input / block_length a in
+  let n = if S.length input % block_length a = 0 && n > 0 then n-1 else n in
+  let padding = pad a (S.length input) in
+  let padded_d = input `S.append` padding in
+  let blocks, rest = Lib.UpdateMulti.split_block (block_length a) padded_d n in
+  let blocks', rest' = S.split input (n * block_length a) in
+  S.lemma_eq_intro blocks blocks';
+  S.lemma_eq_intro (rest' `S.append` padding) rest;
+  Math.Lemmas.multiple_modulo_lemma n (block_length a);
+  S.lemma_eq_intro padded_d (blocks `S.append` rest);
+  update_multi_associative a (init a) blocks rest;
+  S.lemma_eq_intro (fst (update_multi a (init a) padded_d)) (fst (update_multi a (update_multi a (init a) blocks) rest));
+  assert(
+      let kk = 0 in
+      let k = Seq.empty in
+      let d = input in
+      let nn = Spec.Blake2.max_output (to_blake_alg a) in
+      let prev0 = Spec.Blake2.compute_prev0 (to_blake_alg a) kk in
+      let s = Spec.Blake2.blake2_init (to_blake_alg a) kk k nn in
+      (**)
+      s == fst (init a));
+  assert(
+    let bs, l = split_blocks a input in
+    let hash0 = update_multi a (init a) bs in
+    update_last a hash0 (S.length bs) l ==
+      update_last_blake a hash0 (S.length bs) l);
+  let (nb,rem) = split (to_blake_alg a) (Seq.length input) in
+  let s0 = init a in
+  let hash : words_state' a = fst s0 in
+  let prev = v #U64 #SEC (snd s0) in
+//  let s = repeati nb (blake2_update1 a prev m) s in
+  assume(
+    nb * block_length a <= Seq.length input /\
+    prev + nb * block_length a <= max_limb (to_blake_alg a) /\
+    nb < Seq.length input / size_block (to_blake_alg a) /\
+    prev + Seq.length input <= max_limb (to_blake_alg a) /\
+    prev + nb * block_length a <= pow2 64 - 1);
+  repeati_blake2_update1_as_update_multi_eq a nb prev input hash
+
+
+#push-options "--z3rlimit 1000"
+let blake2_is_hash_incremental
+  (a:hash_alg{is_blake a}) (input:bytes{Seq.length input <= max_input_length a})
+  : Lemma
+    (Spec.Blake2.blake2 (to_blake_alg a) input 0 Seq.empty
+                        (Spec.Blake2.max_output (to_blake_alg a)) ==
      hash_incremental a input)
   =
   let open FStar.Mul in
@@ -164,9 +537,70 @@ let blake2_is_hash_incremental
   assert(
     let bs, l = split_blocks a input in
     let hash0 = update_multi a (init a) bs in
-    let hash1 = update_last a hash0 (S.length bs) l in
-    hash1 == update_last_blake a hash0 (S.length bs) l);
+    update_last a hash0 (S.length bs) l ==
+      update_last_blake a hash0 (S.length bs) l);
+  let (nb,rem) = split (to_blake_alg a) (Seq.length input) in
+  let s0 = init a in
+  let hash : words_state' a = fst s0 in
+  let prev = v #U64 #SEC (snd s0) in
+//  let s = repeati nb (blake2_update1 a prev m) s in
+  assume(
+    nb * block_length a <= Seq.length input /\
+    prev + nb * block_length a <= max_limb (to_blake_alg a) /\
+    nb < Seq.length input / size_block (to_blake_alg a) /\
+    prev + Seq.length input <= max_limb (to_blake_alg a) /\
+    prev + nb * block_length a <= pow2 64 - 1);
+  repeati_blake2_update1_as_update_multi_eq a nb prev input hash
+
+repeati_blake2_update1_as_update_multi_eq
+  (a:hash_alg{is_blake a}) (nb prev : nat)
+  (d : bytes)
+  (hash : words_state' a) :
+  Lemma
+  (requires (
+    nb * block_length a <= Seq.length d /\
+    prev + nb * block_length a <= max_limb (to_blake_alg a) /\
+    nb < Seq.length d / size_block (to_blake_alg a) /\
+    prev + Seq.length d <= max_limb (to_blake_alg a) /\
+    prev + nb * block_length a <= pow2 64 - 1
+  ))
+  (ensures (
+    let blocks, _ = Seq.split d (nb * block_length a) in
+    (Loops.repeati nb (blake2_update1 (to_blake_alg a) prev d) hash,
+     u64 (prev + nb * block_length a)) ==
+    update_multi a (hash, u64 prev) blocks)) =
+
+  
+let blake2_update_blocks a prev m s =
+  let (nb,rem) = split a (length m) in
+  let s = repeati nb (blake2_update1 a prev m) s in
+  blake2_update_last a prev rem m s
+  
+
+
+  assume(
+      let kk = 0 in
+      let k = Seq.empty in
+      let d = input in
+      let nn = Spec.Blake2.max_output (to_blake_alg a) in
+      let prev0 = Spec.Blake2.compute_prev0 (to_blake_alg a) kk in
+      let s = Spec.Blake2.blake2_init (to_blake_alg a) kk k nn in
+      let s = Spec.Blake2.blake2_update_blocks (to_blake_alg a) prev0 d s in
+      (**)
+      let bs, l = split_blocks a input in
+      let hash = update_multi a (init a) bs in
+      let hash = update_last a hash (S.length bs) l in
+      s == fst hash);
   admit()
+
+      let s = Spec.Blake2.blake2_init (to_blake_alg a) kk k nn in
+      let s = Spec.Blake2.blake2_update_blocks (to_blake_alg a) prev0 d s in
+
+let blake2_update_blocks a prev m s =
+  let (nb,rem) = split a (length m) in
+  let s = repeati nb (blake2_update1 a prev m) s in
+  blake2_update_last a prev rem m s
+
 
 
 
